new add/carry chain logic with admitted proofs

src/Arithmetic/Saturated.v
@@ -171,93 +171,6 @@ Hint Opaque Associational.mul Associational.multerm : uncps.
 Hint Rewrite @Associational.mul_id @Associational.multerm_id : uncps.
 Hint Rewrite @Associational.eval_mul @Associational.eval_map_multerm using (omega || assumption) : push_basesystem_eval.
 
-Module Positional.
-  Section Positional.
-    Context (weight : nat->Z) {s:Z}. (* s is number at which to split *)
-    Section GenericOp.
-      Context {op : Z -> Z -> Z}
-              {op_get_carry : Z -> Z -> Z * Z} (* no carry in, carry out *)
-              {op_with_carry : Z -> Z -> Z -> Z * Z}. (* carry in, carry out  *)
-
-      Fixpoint chain_op'_cps {n}:
-        option Z->Z^n->Z^n->forall T, (Z*Z^n->T)->T :=
-        match n with
-        | O => fun c p _ _ f =>
-                 let carry := match c with | None => 0 | Some x => x end in
-                 f (carry,p)
-        | S n' =>
-          fun c p q _ f =>
-            (* for the first call, use op_get_carry, then op_with_carry *)
-            let op' := match c with
-                       | None => op_get_carry
-                       | Some x => op_with_carry x end in
-            dlet carry_result := op' (hd p) (hd q) in
-              chain_op'_cps (Some (fst carry_result)) (tl p) (tl q) _
-                            (fun carry_pq =>
-                               f (fst carry_pq,
-                                  append (snd carry_result) (snd carry_pq)))
-        end.
-      Definition chain_op' {n} c p q := @chain_op'_cps n c p q _ id.
-      Definition chain_op_cps {n} p q {T} f := @chain_op'_cps n None p q T f.
-      Definition chain_op {n} p q : Z * Z^n := chain_op_cps p q id.
-
-      Lemma chain_op'_id {n} : forall c p q T f,
-        @chain_op'_cps n c p q T f = f (chain_op' c p q).
-      Proof.
-        cbv [chain_op']; induction n; intros; destruct c;
-          simpl chain_op'_cps; cbv [Let_In]; try reflexivity.
-        { etransitivity; rewrite IHn; reflexivity. }
-        { etransitivity; rewrite IHn; reflexivity. }
-      Qed.
-
-      Lemma chain_op_id {n} p q T f :
-        @chain_op_cps n p q T f = f (chain_op p q).
-      Proof. apply chain_op'_id. Qed.
-    End GenericOp.
-
-    Section AddSub.
-      Local Definition eval {n} := B.Positional.eval (n:=n) weight.
-      
-      Definition sat_add_cps {n} p q T (f:Z*Z^n->T) :=
-        chain_op_cps (op_get_carry := Z.add_get_carry_full s)
-                     (op_with_carry := Z.add_with_get_carry_full s)
-                     p q f.
-      Definition sat_add {n} p q := @sat_add_cps n p q _ id.
-
-      Lemma sat_add_id n p q T f :
-        @sat_add_cps n p q T f = f (sat_add p q).
-      Proof. cbv [sat_add sat_add_cps]. rewrite !chain_op_id. reflexivity. Qed.
-
-      Lemma sat_add_mod n p q :
-        eval (snd (@sat_add n p q)) = (eval p + eval q) mod s.
-      Admitted.
-
-      Lemma sat_add_div n p q :
-        fst (@sat_add n p q) = (eval p + eval q) / s.
-      Admitted.
-      
-      Definition sat_sub_cps {n} p q T (f:Z*Z^n->T) :=
-        chain_op_cps (op_get_carry := Z.sub_get_borrow_full s)
-                     (op_with_carry := Z.sub_with_get_borrow_full s)
-                     p q f.
-      Definition sat_sub {n} p q := @sat_sub_cps n p q _ id.
-
-      Lemma sat_sub_id n p q T f :
-        @sat_sub_cps n p q T f = f (sat_sub p q).
-      Proof. cbv [sat_sub sat_sub_cps]. rewrite !chain_op_id. reflexivity. Qed.
-
-      Lemma sat_sub_mod n p q :
-        eval (snd (@sat_sub n p q)) = (eval p - eval q) mod s.
-      Admitted.
-
-      Lemma sat_sub_div n p q :
-        fst (@sat_sub n p q) = - ((eval p - eval q) / s).
-      Admitted.
-                 
-    End Add.
-  End Positional.
-End Positional.
-
 
 Module Columns.
   Section Columns.
@@ -795,7 +708,107 @@ Section UniformWeight.
     ring.
   Qed.
 
+  Definition small {n} (p : Z^n) : Prop :=
+    forall x, In x (to_list _ p) -> 0 <= x < bound.
+
 End UniformWeight.
+
+Module Positional.
+  Section Positional.
+    Context {s:Z}. (* s is bitwidth *)
+    Let small {n} := @small s n.
+    Section GenericOp.
+      Context {op : Z -> Z -> Z}
+              {op_get_carry : Z -> Z -> Z * Z} (* no carry in, carry out *)
+              {op_with_carry : Z -> Z -> Z -> Z * Z}. (* carry in, carry out  *)
+
+      Fixpoint chain_op'_cps {n}:
+        option Z->Z^n->Z^n->forall T, (Z*Z^n->T)->T :=
+        match n with
+        | O => fun c p _ _ f =>
+                 let carry := match c with | None => 0 | Some x => x end in
+                 f (carry,p)
+        | S n' =>
+          fun c p q _ f =>
+            (* for the first call, use op_get_carry, then op_with_carry *)
+            let op' := match c with
+                       | None => op_get_carry
+                       | Some x => op_with_carry x end in
+            dlet carry_result := op' (hd p) (hd q) in
+              chain_op'_cps (Some (fst carry_result)) (tl p) (tl q) _
+                            (fun carry_pq =>
+                               f (fst carry_pq,
+                                  append (snd carry_result) (snd carry_pq)))
+        end.
+      Definition chain_op' {n} c p q := @chain_op'_cps n c p q _ id.
+      Definition chain_op_cps {n} p q {T} f := @chain_op'_cps n None p q T f.
+      Definition chain_op {n} p q : Z * Z^n := chain_op_cps p q id.
+
+      Lemma chain_op'_id {n} : forall c p q T f,
+        @chain_op'_cps n c p q T f = f (chain_op' c p q).
+      Proof.
+        cbv [chain_op']; induction n; intros; destruct c;
+          simpl chain_op'_cps; cbv [Let_In]; try reflexivity.
+        { etransitivity; rewrite IHn; reflexivity. }
+        { etransitivity; rewrite IHn; reflexivity. }
+      Qed.
+
+      Lemma chain_op_id {n} p q T f :
+        @chain_op_cps n p q T f = f (chain_op p q).
+      Proof. apply chain_op'_id. Qed.
+    End GenericOp.
+
+    Section AddSub.
+      Let eval {n} := B.Positional.eval (n:=n) (uweight s).
+      
+      Definition sat_add_cps {n} p q T (f:Z*Z^n->T) :=
+        chain_op_cps (op_get_carry := Z.add_get_carry_full s)
+                     (op_with_carry := Z.add_with_get_carry_full s)
+                     p q f.
+      Definition sat_add {n} p q := @sat_add_cps n p q _ id.
+
+      Lemma sat_add_id n p q T f :
+        @sat_add_cps n p q T f = f (sat_add p q).
+      Proof. cbv [sat_add sat_add_cps]. rewrite !chain_op_id. reflexivity. Qed.
+
+      Lemma sat_add_mod n p q :
+        eval (snd (@sat_add n p q)) = (eval p + eval q) mod (uweight s n).
+      Admitted.
+
+      Lemma sat_add_div n p q :
+        fst (@sat_add n p q) = (eval p + eval q) / (uweight s n).
+      Admitted.
+
+      Lemma small_sat_add n p q : small (snd (@sat_add n p q)).
+      Admitted.
+      
+      Definition sat_sub_cps {n} p q T (f:Z*Z^n->T) :=
+        chain_op_cps (op_get_carry := Z.sub_get_borrow_full s)
+                     (op_with_carry := Z.sub_with_get_borrow_full s)
+                     p q f.
+      Definition sat_sub {n} p q := @sat_sub_cps n p q _ id.
+
+      Lemma sat_sub_id n p q T f :
+        @sat_sub_cps n p q T f = f (sat_sub p q).
+      Proof. cbv [sat_sub sat_sub_cps]. rewrite !chain_op_id. reflexivity. Qed.
+
+      Lemma sat_sub_mod n p q :
+        eval (snd (@sat_sub n p q)) = (eval p - eval q) mod (uweight s n).
+      Admitted.
+
+      Lemma sat_sub_div n p q :
+        fst (@sat_sub n p q) = - ((eval p - eval q) / uweight s n).
+      Admitted.
+
+      Lemma small_sat_sub n p q : small (snd (@sat_sub n p q)).
+      Admitted.
+                 
+    End AddSub.
+  End Positional.
+End Positional.
+Hint Opaque Positional.sat_sub Positional.sat_add Positional.chain_op Positional.chain_op' : uncps.
+Hint Rewrite @Positional.sat_sub_id @Positional.sat_add_id @Positional.chain_op_id @Positional.chain_op' : uncps.
+Hint Rewrite @Positional.sat_sub_mod @Positional.sat_sub_div @Positional.sat_add_mod @Positional.sat_add_div using (omega || assumption) : push_basesystem_eval.
 
 Section API.
   Context (bound : Z) {bound_pos : bound > 0}.
@@ -804,8 +817,7 @@ Section API.
   (* lowest limb is less than its bound; this is required for [divmod]
   to simply separate the lowest limb from the rest and be equivalent
   to normal div/mod with [bound]. *)
-  Definition small {n} (p : T n) : Prop :=
-    forall x, In x (to_list _ p) -> 0 <= x < bound.
+  Local Notation small := (@small bound).
 
   Definition zero {n:nat} : T n := B.Positional.zeros n.
 
@@ -835,21 +847,33 @@ Section API.
       (fun carry_result =>f (snd carry_result)).
   Definition scmul {n} c p : T (S n) := @scmul_cps n c p _ id.
 
-  Definition add_cps {n m pred_nm} (p : T n) (q : T m) {R} (f:T (S pred_nm)->R) :=
-    Columns.add_cps (uweight bound) p q
-      (fun carry_result => Tuple.left_append_cps (fst carry_result) (snd carry_result)
-      f).
-  Definition add {n m pred_nm} p q : T (S pred_nm) := @add_cps n m pred_nm p q _ id.
+  Definition add_cps {n} (p q: T n) {R} (f:T n->R) :=
+    Positional.sat_add_cps (s:=bound) p q _
+      (* drops last carry, this relies on bounds *)
+      (fun carry_result => f (snd carry_result)).
+  Definition add {n} p q : T n := @add_cps n p q _ id.
 
-  Definition sub_then_maybe_add_cps {n} mask (p q r : T n) {R} (f:T n -> R) :=
-    Columns.unbalanced_sub_cps (n3:=n) (uweight bound) p q
+  (* Wrappers for additions with slightly uneven limb counts *)
+  Definition add_S1_cps {n} (p: T (S n)) (q: T n) {R} (f:T (S n)->R) :=
+    join0_cps q (fun Q => add_cps p Q f).
+  Definition add_S1 {n} p q := @add_S1_cps n p q _ id. 
+  Definition add_S2_cps {n} (p: T n) (q: T (S n)) {R} (f:T (S n)->R) :=
+    join0_cps p (fun P => add_cps P q f).
+  Definition add_S2 {n} p q := @add_S2_cps n p q _ id. 
+
+  Definition sub_then_maybe_add_cps {n} mask (p q r : T n)
+             {R} (f:T n -> R) :=
+    Positional.sat_sub_cps (s:=bound) p q _
       (* the carry will be 0 unless we underflow--we do the addition only
          in the underflow case *)
       (fun carry_result =>
-         Columns.conditional_add_cps (uweight bound) mask (fst carry_result) (left_append (fst carry_result) (snd carry_result)) r
-      (* We can now safely discard the carry. This relies on the
-         precondition that p - q + r < bound^n. *)
-      (fun carry_result' => f (snd carry_result'))).
+         B.Positional.select_cps mask (fst carry_result) r
+      (fun selected => join0_cps selected
+      (fun selected' =>
+         Positional.sat_sub_cps (s:=bound) (left_append (fst carry_result) (snd carry_result)) selected' _
+      (* We can now safely discard the carry and the highest digit.
+         This relies on the precondition that p - q + r < bound^n. *)
+      (fun carry_result' => drop_high_cps (snd carry_result') f)))).
   Definition sub_then_maybe_add {n} mask (p q r : T n) :=
     sub_then_maybe_add_cps mask p q r id.
 
@@ -857,14 +881,15 @@ Section API.
     that 0 <= p < 2*q and q < bound^n (this ensures the output is less
     than bound^n). *)
   Definition conditional_sub_cps {n} (p:Z^S n) (q:Z^n) R (f:Z^n->R) :=
-    Columns.unbalanced_sub_cps (n3:=S n) (uweight bound) p q
+    join0_cps q
+    (fun qq => Positional.sat_sub_cps (s:=bound) p qq _
       (* if carry is zero, we select the result of the subtraction,
       otherwise the first input *)
       (fun carry_result =>
         Tuple.map2_cps (Z.zselect (fst carry_result)) (snd carry_result) p
       (* in either case, since our result must be < q and therefore <
       bound^n, we can drop the high digit *)
-      (fun r => drop_high_cps r f)).
+      (fun r => drop_high_cps r f))).
   Definition conditional_sub {n} p q := @conditional_sub_cps n p q _ id.
 
   Hint Opaque join0 divmod drop_high scmul add sub_then_maybe_add conditional_sub : uncps.
@@ -894,17 +919,26 @@ Section API.
       @scmul_cps n c p R f = f (scmul c p).
     Proof. cbv [scmul_cps scmul]. prove_id. Qed.
 
-    Lemma add_id n m pred_nm p q R f :
-      @add_cps n m pred_nm p q R f = f (add p q).
+    Lemma add_id n p q R f :
+      @add_cps n p q R f = f (add p q).
     Proof. cbv [add_cps add Let_In]. prove_id. Qed.
+    Hint Rewrite add_id : uncps.
+    
+    Lemma add_S1_id n p q R f :
+      @add_S1_cps n p q R f = f (add_S1 p q).
+    Proof. cbv [add_S1_cps add_S1 join0_cps]. prove_id. Qed.
+    
+    Lemma add_S2_id n p q R f :
+      @add_S2_cps n p q R f = f (add_S2 p q).
+    Proof. cbv [add_S2_cps add_S2 join0_cps]. prove_id. Qed.
 
     Lemma sub_then_maybe_add_id n mask p q r R f :
       @sub_then_maybe_add_cps n mask p q r R f = f (sub_then_maybe_add mask p q r).
-    Proof. cbv [sub_then_maybe_add_cps sub_then_maybe_add Let_In]. prove_id. Qed.
+    Proof. cbv [sub_then_maybe_add_cps sub_then_maybe_add join0_cps Let_In]. prove_id. Qed.
 
     Lemma conditional_sub_id n p q R f :
       @conditional_sub_cps n p q R f = f (conditional_sub p q).
-    Proof. cbv [conditional_sub_cps conditional_sub Let_In]. prove_id. Qed.
+    Proof. cbv [conditional_sub_cps conditional_sub join0_cps Let_In]. prove_id. Qed.
 
   End CPSProofs.
   Hint Rewrite nonzero_id join0_id divmod_id drop_high_id scmul_id add_id sub_then_maybe_add_id conditional_sub_id : uncps.
@@ -1005,13 +1039,13 @@ Section API.
       pose proof Z.mul_split_div; pose proof Z.mul_split_mod;
       pose proof div_correct; pose proof modulo_correct.
 
-    Lemma eval_add_nz n m pred_nm p q :
-      pred_nm <> 0%nat ->
-      eval (@add n m pred_nm p q) = eval p + eval q.
+    Lemma eval_add_nz n p q :
+      n <> 0%nat -> (0 <= eval p + eval q < uweight bound n) ->
+      eval (@add n p q) = eval p + eval q.
     Proof.
       intros. pose_all.
       repeat match goal with
-             | _ => progress (cbv [add_cps add eval Let_In]; repeat autounfold)
+             | _ => progress (cbv [add_cps add eval Let_In] in *; repeat autounfold)
              | _ => progress autorewrite with uncps push_id cancel_pair push_basesystem_eval
              | _ => rewrite B.Positional.eval_left_append
 
@@ -1019,33 +1053,36 @@ Section API.
                       (rewrite <-!from_list_default_eq with (d:=0);
                        erewrite !length_to_list, !from_list_default_eq,
                        from_list_to_list)
-             | _ => rewrite Z.mul_div_eq by auto;
-                      omega
+             | _ => apply Z.mod_small; omega 
              end.
     Qed.
 
-    Lemma eval_add_z n m pred_nm p q :
-      pred_nm = 0%nat ->
+    Lemma eval_add_z n p q :
       n = 0%nat ->
-      m = 0%nat ->
-      eval (@add n m pred_nm p q) = eval p + eval q.
+      eval (@add n p q) = eval p + eval q.
     Proof. intros; subst; reflexivity. Qed.
 
-    Lemma eval_add n m pred_nm p q (Hpred_nm : pred_nm = 0%nat -> n = 0%nat /\ m = 0%nat)
-      :  eval (@add n m pred_nm p q) = eval p + eval q.
+    Lemma eval_add n p q (H:0 <= eval p + eval q < uweight bound n)
+      :  eval (@add n p q) = eval p + eval q.
     Proof.
-      destruct (Nat.eq_dec pred_nm 0%nat); intuition auto using eval_add_z, eval_add_nz.
+      destruct (Nat.eq_dec n 0%nat); intuition auto using eval_add_z, eval_add_nz.
     Qed.
-    Lemma eval_add_same n p q
-      :  eval (@add n n n p q) = eval p + eval q.
+    Lemma eval_add_same n p q (H:0 <= eval p + eval q < uweight bound n)
+      :  eval (@add n p q) = eval p + eval q.
     Proof. apply eval_add; omega. Qed.
-    Lemma eval_add_S1 n p q
-      :  eval (@add (S n) n (S n) p q) = eval p + eval q.
-    Proof. apply eval_add; omega. Qed.
-    Lemma eval_add_S2 n p q
-      :  eval (@add n (S n) (S n) p q) = eval p + eval q.
-    Proof. apply eval_add; omega. Qed.
-    Hint Rewrite eval_add_same eval_add_S1 eval_add_S2 : push_basesystem_eval.
+    Lemma eval_add_S1 n p q (H:0 <= eval p + eval q < uweight bound (S n))
+      :  eval (@add_S1 n p q) = eval p + eval q.
+    Proof.
+      cbv [add_S1 add_S1_cps]. autorewrite with uncps push_id.
+      rewrite eval_add; rewrite eval_join0; [reflexivity|assumption].
+    Qed.
+    Lemma eval_add_S2 n p q (H:0 <= eval p + eval q < uweight bound (S n))
+      :  eval (@add_S2 n p q) = eval p + eval q.
+    Proof.
+      cbv [add_S2 add_S2_cps]. autorewrite with uncps push_id.
+      rewrite eval_add; rewrite eval_join0; [reflexivity|assumption].
+    Qed.
+    Hint Rewrite eval_add_same eval_add_S1 eval_add_S2 using (omega || assumption): push_basesystem_eval.
 
     Lemma uweight_le_mono n m : (n <= m)%nat ->
       uweight bound n <= uweight bound m.
@@ -1104,43 +1141,15 @@ Section API.
         apply Z.mod_pos_bound, Z.gt_lt, bound_pos. }
     Qed.
 
-    Lemma small_add n m pred_nm a b :
-      (2 <= bound) -> (max n m <= pred_nm)%nat ->
-      small a -> small b -> small (@add n m pred_nm a b).
+    Lemma small_add n a b :
+      (2 <= bound) -> 
+      small a -> small b -> small (@add n a b).
     Proof.
       intros. pose_all.
-      cbv [small add_cps add Let_In]. repeat autounfold.
+      cbv [add_cps add Let_In].
       autorewrite with uncps push_id.
-      rewrite Tuple.to_list_left_append.
-      let H := fresh "H" in intros x H; apply in_app_or in H;
-                              destruct H as [H | H];
-                              [apply (small_compact _ _ H)
-                              |destruct H; [|exfalso; assumption] ].
-      subst x.
-      rewrite Columns.compact_div by assumption.
-      repeat match goal with
-               H : small ?x |- _ => apply eval_small in H; cbv [eval] in H
-             end.
-      destruct pred_nm as [|pred_pred_nm]; autorewrite with push_basesystem_eval;
-        repeat match goal with
-               | [ H : (max ?x ?y <= 0)%nat |- _ ]
-                 => assert (x = 0%nat) by omega *;
-                      assert (y = 0%nat) by omega *;
-                      clear H
-               | _ => progress subst
-               end.
-      { destruct bound; cbv -[Z.le Z.lt]; lia. }
-      split; [ solve [ unfold uweight in *; Z.zero_bounds ] | ].
-      apply Zdiv_lt_upper_bound; [ solve [ unfold uweight in *; Z.zero_bounds ] | ].
-      apply Z.lt_le_trans with (m:=uweight bound n + uweight bound m);
-          [omega|].
-      apply Z.le_trans with (m:=uweight bound (max n m) + uweight bound (max n m)); auto using Z.add_le_mono, uweight_le_mono, Max.le_max_l, Max.le_max_r.
-      rewrite Z.add_diag.
-      pose proof (uweight_le_mono (max n m) (S pred_pred_nm)).
-      specialize_by_assumption.
-      apply Z.mul_le_mono_nonneg; try omega.
-      apply Max.max_case_strong; omega.
-    Qed.
+      apply Positional.small_sat_add.
+    Admitted.
 
     Lemma small_left_tl n (v:T (S n)) : small v -> small (left_tl v).
     Proof. cbv [small]. auto using Tuple.In_to_list_left_tl. Qed.
@@ -1190,29 +1199,22 @@ Section API.
              | _ => progress (cbv [sub_then_maybe_add sub_then_maybe_add_cps eval] in *; intros)
              | _ => progress autounfold
              | _ => progress autorewrite with uncps push_id push_basesystem_eval
+             | _ => rewrite eval_drop_high
+             | _ => rewrite eval_join0
              | H : small _ |- _ => apply eval_small in H
              | _ => progress break_match
              | _ => (rewrite Z.add_opp_r in * )
-             | _ => progress autorewrite with zsimplify; [ ]
              | H : _ |- _ => rewrite Z.ltb_lt in H;
                                rewrite <-div_nonzero_neg_iff with
                                (y:=uweight bound n) in H by (auto; omega)
              | H : _ |- _ => rewrite Z.ltb_ge in H
              | _ => rewrite Z.mod_small by omega
              | _ => omega
-             end;
-      repeat match goal with
-             | H : _ |- _ => rewrite div_nonzero_neg_iff in H
-                 by (auto; omega)
-             | |- context [-?x + ?y mod ?x] =>
-               replace (-x + y mod x) with y
-                 by (rewrite Z.mod_eq, Z.div_small_neg; omega)
-             | _ => apply Z.mod_small; omega
-             | _ => omega
+             | _ => progress autorewrite with zsimplify; [ ]
              end.
-    Qed.
+    Admitted.
 
-    Lemma eval_sub_then_maybe_add n mask p q r:
+    Lemma eval_sub_then_maybe_add n mask p q r :
       small p -> small q -> small r ->
       (map (Z.land mask) r = r) ->
       (0 <= eval p < eval r) -> (0 <= eval q < eval r) ->
@@ -1227,7 +1229,7 @@ Section API.
    Proof.
      cbv [sub_then_maybe_add_cps sub_then_maybe_add]; intros.
      repeat progress autounfold. autorewrite with uncps push_id.
-     apply small_compact.
+     apply small_drop_high, Positional.small_sat_sub.
    Qed.
 
    (* TODO : remove if unneeded when all admits are proven
@@ -1277,12 +1279,13 @@ Section API.
                | _ => progress cbv [eval]
                | H : (_ <=? _) = true |- _ => apply Z.leb_le in H
                | H : (_ <=? _) = false |- _ => apply Z.leb_gt in H
-               | _ => rewrite eval_drop_high by auto using small_compact
+               | _ => rewrite eval_drop_high by auto using Positional.small_sat_sub
+               | _ => (rewrite eval_join0 in * )
                | _ => progress autorewrite with uncps push_id push_basesystem_eval
-               | _ => rewrite Z.mod_small by (rewrite ?Z.mod_small; omega)
+               | _ => repeat rewrite Z.mod_small; omega
                | _ => omega
                end.
-   Qed.
+    Admitted.
 
     Lemma eval_conditional_sub n (p:T (S n)) (q:T n)
            (psmall : small p) (qsmall : small q) :
